theories/semantics/semantics.v
@@ -1,7 +1,7 @@
 (* This file summarizes the content of the semantics/ directory. *)
 
 From osiris.semantics Require Export
-  free
+  micro
   code
   eval
   step
